Steel.PCM.Effect.Atomic

pulse/ulib/experimental/Steel.PCM.Heap.fst
@@ -829,3 +829,50 @@ let extend #a #pcm x addr h =
      in
      (| r, h' |)
 #pop-options
+
+
+let frame (#a:Type)
+          (#pre:slprop)
+          (#post:a -> slprop)
+          (frame:slprop)
+          ($f:action pre a post)
+  = let g : refined_pre_action (pre `star` frame) a (fun x -> post x `star` frame)
+        = fun h0 ->
+              assert (interp (pre `star` frame) h0);
+              affine_star pre frame h0;
+              let (| x, h1 |) = f h0 in
+              assert (interp (post x) h1);
+              assert (interp (post x `star` frame) h1);
+              assert (forall frame'. frame_related_heaps h0 h1 pre (post x) frame' false);
+              let aux (frame':slprop)
+                : Lemma (requires
+                            interp ((pre `star` frame) `star` frame') h0)
+                        (ensures
+                            interp ((post x `star` frame) `star` frame') h1)
+                        [SMTPat ()]
+                = star_associative pre frame frame';
+                  star_associative (post x) frame frame'
+              in
+              assert (forall frame'. frame_related_heaps h0 h1 (pre `star` frame) (post x `star` frame) frame' false);
+              (| x, h1 |)
+    in
+    refined_pre_action_as_action g
+
+let change_slprop (p q:slprop)
+                  (proof: (h:heap -> Lemma (requires interp p h) (ensures interp q h)))
+  : action p unit (fun _ -> q)
+  = let g
+      : refined_pre_action p unit (fun _ -> q)
+      = fun h ->
+          proof h;
+          let aux (frame:slprop)
+            : Lemma (requires
+                        interp (p `star` frame) h)
+                    (ensures
+                        interp (q `star` frame) h)
+                    [SMTPat ()]
+            = FStar.Classical.forall_intro (FStar.Classical.move_requires proof)
+          in
+          (| (), h |)
+    in
+    refined_pre_action_as_action g
